add tests

Test/git-issues/git-issue-2500.dfy
@@ -1,22 +1,24 @@
 // RUN: %exits-with 4 %dafny /compile:0 "%s" > "%t"
 // RUN: %diff "%s.expect" "%t"
 
-module A {
-  trait {:termination false} Trait {
-    function TotallyNotZero() : (ret: int)
-      ensures ret != 0
+module M {
+  trait {:termination false} Tr {
+    function True(): (ret: bool) ensures ret
+    function True'(): (ret: bool) ensures True'()
+    function Other(x:nat, free: Tr): bool
+      ensures x != 0 && free.Other(x-1, free) ==> Other(x-1, free)
   }
 }
 
-module B {
-  import opened A
-
-  class Class extends Trait {
-    constructor() {}
-    function TotallyNotZero() : (ret: int)
-      // Missing: ensures ret != 0
-    { 
-      0 
-    }
-  }
+class Class extends M.Tr {
+  function True(): (ret: bool)
+    // Missing: ensures ret != 0
+  { false }
+  function True'(): (ret: bool)
+    // Missing: ensures True'()
+  { false }
+  function Other(x: nat, free: M.Tr): bool
+    // Different Receiver
+    ensures x != 0 && Other(x-1, free) ==> Other(x-1, free)
+  { false }
 }
